updates
Signed-off-by: Shaobo He <shaobohe@amazon.com>

cedar-lean/Cedar/Thm/Validation/WellTyped.lean
@@ -13,257 +13,268 @@
  See the License for the specific language governing permissions and
  limitations under the License.
 -/
-import Cedar.Validation.TypedExpr
-import Cedar.Thm
-import Cedar.Spec.Ext
+
+import Cedar.Thm.Validation.WellTyped.Definition
+import Cedar.Thm.Validation.WellTyped.TypeLifting
 
 /-!
-This file contains useful definitions and lemmas about well-typedness of `TypedExpr`
+This file contains well-typedness theorems of `TypedExpr`
 -/
-
-namespace Cedar.Spec
-
-open Cedar.Validation
-open Cedar.Spec.Ext
-
-inductive Prim.WellTyped (env : Environment) : Prim → CedarType → Prop
-  | bool (b : Bool) :
-    WellTyped env (.bool b) (.bool .anyBool)
-  | int (i : Int64) :
-    WellTyped env (.int i) .int
-  | string (s : String) :
-    WellTyped env (.string s) .string
-  | entityUID (uid : EntityUID)
-    (h₁ : env.ets.isValidEntityUID uid || env.acts.contains uid) :
-    WellTyped env (.entityUID uid) (.entity uid.ty)
-
-inductive Var.WellTyped (env : Environment) : Var → CedarType → Prop
-  | principal :
-    WellTyped env .principal (.entity env.reqty.principal)
-  | resource :
-    WellTyped env .resource (.entity env.reqty.resource)
-  | action :
-    WellTyped env .action (.entity env.reqty.action.ty)
-  | context:
-    WellTyped env .context (.record env.reqty.context)
-
-inductive UnaryOp.WellTyped : UnaryOp → TypedExpr → CedarType → Prop
-  | not {x₁ : TypedExpr}
-    (h₁ : x₁.typeOf = .bool .anyBool) :
-    WellTyped .not x₁ (.bool .anyBool)
-  | neg {x₁ : TypedExpr}
-    (h₁ : x₁.typeOf = .int) :
-    WellTyped .neg x₁ .int
-  | isEmpty {x₁ : TypedExpr} {eltTy : CedarType}
-    (h₁ : x₁.typeOf = .set eltTy) :
-    WellTyped .isEmpty x₁ (.bool .anyBool)
-  | like {x₁ : TypedExpr} {p : Pattern}
-    (h₁ : x₁.typeOf = .string) :
-    WellTyped (.like p) x₁ (.bool .anyBool)
-
-inductive BinaryOp.WellTyped (env : Environment) : BinaryOp → TypedExpr → TypedExpr → CedarType → Prop
-  | eq {x₁ x₂ : TypedExpr}
-    (h₁ : x₁.typeOf = x₂.typeOf) :
-    WellTyped env .eq x₁ x₂ (.bool .anyBool)
-  | memₑ {x₁ x₂ : TypedExpr} {ety₁ ety₂ : EntityType}
-    (h₁ : x₁.typeOf = .entity ety₁)
-    (h₂ : x₂.typeOf = .entity ety₁) :
-    WellTyped env .mem x₁ x₂ (.bool .anyBool)
-  | memₛ {x₁ x₂ : TypedExpr} {ety₁ ety₂ : EntityType}
-    (h₁ : x₁.typeOf = .entity ety₁)
-    (h₂ : x₂.typeOf = .set (.entity ety₁)) :
-    WellTyped env .mem x₁ x₂ (.bool .anyBool)
-  | less_int {x₁ x₂ : TypedExpr}
-    (h₁ : x₁.typeOf = .int)
-    (h₂ : x₂.typeOf = .int) :
-    WellTyped env .less x₁ x₂ (.bool .anyBool)
-  | less_datetime {x₁ x₂ : TypedExpr}
-    (h₁ : x₁.typeOf = .ext .datetime)
-    (h₂ : x₂.typeOf = .ext .datetime) :
-    WellTyped env .less x₁ x₂ (.bool .anyBool)
-  | less_duration {x₁ x₂ : TypedExpr}
-    (h₁ : x₁.typeOf = .ext .duration)
-    (h₂ : x₂.typeOf = .ext .duration) :
-    WellTyped env .less x₁ x₂ (.bool .anyBool)
-  | lessEq_int {x₁ x₂ : TypedExpr}
-    (h₁ : x₁.typeOf = .int)
-    (h₂ : x₂.typeOf = .int) :
-    WellTyped env .lessEq x₁ x₂ (.bool .anyBool)
-  | lessEq_datetime {x₁ x₂ : TypedExpr}
-    (h₁ : x₁.typeOf = .ext .datetime)
-    (h₂ : x₂.typeOf = .ext .datetime) :
-    WellTyped env .lessEq x₁ x₂ (.bool .anyBool)
-  | lessEq_duration {x₁ x₂ : TypedExpr}
-    (h₁ : x₁.typeOf = .ext .duration)
-    (h₂ : x₂.typeOf = .ext .duration) :
-    WellTyped env .lessEq x₁ x₂ (.bool .anyBool)
-  | add {x₁ x₂ : TypedExpr}
-    (h₁ : x₁.typeOf = .int)
-    (h₂ : x₂.typeOf = .int) :
-    WellTyped env .add x₁ x₂ .int
-  | sub {x₁ x₂ : TypedExpr}
-    (h₁ : x₁.typeOf = .int)
-    (h₂ : x₂.typeOf = .int) :
-    WellTyped env .sub x₁ x₂ .int
-  | mul {x₁ x₂ : TypedExpr}
-    (h₁ : x₁.typeOf = .int)
-    (h₂ : x₂.typeOf = .int) :
-    WellTyped env .mul x₁ x₂ .int
-  | contains {x₁ x₂ : TypedExpr}
-    (h₁ : x₁.typeOf = .set x₂.typeOf) :
-    WellTyped env .contains x₁ x₂ (.bool .anyBool)
-  | containsAll {x₁ x₂ : TypedExpr} {ty : CedarType}
-    (h₁ : x₁.typeOf = .set ty)
-    (h₂ : x₂.typeOf = .set ty) :
-    WellTyped env .containsAll x₁ x₂ (.bool .anyBool)
-  | containsAny {x₁ x₂ : TypedExpr} {ty : CedarType}
-    (h₁ : x₁.typeOf = .set ty)
-    (h₂ : x₂.typeOf = .set ty) :
-    WellTyped env .containsAny x₁ x₂ (.bool .anyBool)
-  | hasTag {x₁ x₂ : TypedExpr} {ety : EntityType}
-    (h₁ : x₁.typeOf = .entity ety)
-    (h₂ : x₂.typeOf = .string) :
-    WellTyped env .hasTag x₁ x₂ (.bool .anyBool)
-  | getTag {x₁ x₂ : TypedExpr} {ety : EntityType}
-    (h₁ : x₁.typeOf = .entity ety)
-    (h₂ : x₂.typeOf = .string)
-    (h₃ : env.ets.tags? ety = .some (.some ty)) :
-    WellTyped env .getTag x₁ x₂ ty
-
-inductive ExtFun.WellTyped : ExtFun → List TypedExpr → CedarType → Prop
-  | decimal {s₁ : String} {d₁ : Decimal}
-    (h₁ : d₁ = Decimal.decimal s₁) :
-    WellTyped .decimal [.lit (.string s₁) .string] (.ext .decimal)
-  | lessThan {x₁ x₂ : TypedExpr}
-    (h₁ : x₁.typeOf = .ext .decimal)
-    (h₂ : x₂.typeOf = .ext .decimal) :
-    WellTyped .lessThan [x₁, x₂] (.bool .anyBool)
-  | lessThanOrEqual {x₁ x₂ : TypedExpr}
-    (h₁ : x₁.typeOf = .ext .decimal)
-    (h₂ : x₂.typeOf = .ext .decimal) :
-    WellTyped .lessThan [x₁, x₂] (.bool .anyBool)
-  | greaterThan {x₁ x₂ : TypedExpr}
-    (h₁ : x₁.typeOf = .ext .decimal)
-    (h₂ : x₂.typeOf = .ext .decimal) :
-    WellTyped .lessThan [x₁, x₂] (.bool .anyBool)
-  | greaterThanOrEqual {x₁ x₂ : TypedExpr}
-    (h₁ : x₁.typeOf = .ext .decimal)
-    (h₂ : x₂.typeOf = .ext .decimal) :
-    WellTyped .lessThan [x₁, x₂] (.bool .anyBool)
-  | ip {s₁ : String} {ip₁ : IPAddr}
-    (h₁ : ip₁ =  IPAddr.ip s₁) :
-    WellTyped .ip [.lit (.string s₁) .string] (.ext .ipAddr)
-  | isIpv4 {x₁ : TypedExpr}
-    (h₁ : x₁.typeOf = .ext .ipAddr) :
-    WellTyped .isIpv4 [x₁] (.bool .anyBool)
-  | isIpv6 {x₁ : TypedExpr}
-    (h₁ : x₁.typeOf = .ext .ipAddr) :
-    WellTyped .isIpv6 [x₁] (.bool .anyBool)
-  | isLoopback {x₁ : TypedExpr}
-    (h₁ : x₁.typeOf = .ext .ipAddr) :
-    WellTyped .isLoopback [x₁] (.bool .anyBool)
-  | isMulticast {x₁ : TypedExpr}
-    (h₁ : x₁.typeOf = .ext .ipAddr) :
-    WellTyped .isMulticast [x₁] (.bool .anyBool)
-  | isInRange {x₁ x₂ : TypedExpr}
-    (h₁ : x₁.typeOf = .ext .ipAddr)
-    (h₂ : x₂.typeOf = .ext .ipAddr):
-    WellTyped .isInRange [x₁, x₂] (.bool .anyBool)
-  | datetime {s₁ : String} {d₁ : Datetime}
-    (h₁ : d₁ =  Datetime.parse s₁) :
-    WellTyped .datetime [.lit (.string s₁) .string] (.ext .datetime)
-  | duration {s₁ : String} {d₁ : Duration}
-    (h₁ : d₁ =  Datetime.Duration.parse s₁) :
-    WellTyped .duration [.lit (.string s₁) .string] (.ext .duration)
-  | offset {x₁ x₂ : TypedExpr}
-    (h₁ : x₁.typeOf = .ext .datetime)
-    (h₂ : x₂.typeOf = .ext .duration):
-    WellTyped .offset [x₁, x₂] (.ext .datetime)
-  | durationSince {x₁ x₂ : TypedExpr}
-    (h₁ : x₁.typeOf = .ext .datetime)
-    (h₂ : x₂.typeOf = .ext .datetime):
-    WellTyped .durationSince [x₁, x₂] (.ext .duration)
-  | toDate {x₁ : TypedExpr}
-    (h₁ : x₁.typeOf = .ext .datetime) :
-    WellTyped .toDate [x₁] (.ext .datetime)
-  | toTime {x₁ : TypedExpr}
-    (h₁ : x₁.typeOf = .ext .datetime) :
-    WellTyped .toTime [x₁] (.ext .duration)
-
-end Cedar.Spec
 
 namespace Cedar.Thm
 
+open Cedar.Thm
 open Cedar.Validation
 open Cedar.Spec
-open Cedar.Data
 
-inductive TypedExpr.WellTyped (env : Environment) : TypedExpr → Prop
-| lit {p : Prim} {ty : CedarType}
-  (h₁ : p.WellTyped env ty) :
-  WellTyped env (.lit p ty)
-| var {v : Var} {ty : CedarType}
-  (h₁ : v.WellTyped env ty) :
-  WellTyped env (.var v ty)
-| ite {x₁ x₂ x₃ : TypedExpr}
-  (h₁ : WellTyped env x₁)
-  (h₂ : WellTyped env x₂)
-  (h₃ : WellTyped env x₃)
-  (h₄ : x₁.typeOf = .bool .anyBool)
-  (h₅ : x₂.typeOf = x₃.typeOf) :
-  WellTyped env (.ite x₁ x₂ x₃ x₂.typeOf)
-| and {x₁ x₂ : TypedExpr}
-  (h₁ : WellTyped env x₁)
-  (h₂ : WellTyped env x₂)
-  (h₃ : x₁.typeOf = .bool .anyBool)
-  (h₄ : x₂.typeOf = .bool .anyBool) :
-  WellTyped env (.and x₁ x₂ (.bool .anyBool))
-| or {x₁ x₂ : TypedExpr}
-  (h₁ : WellTyped env x₁)
-  (h₂ : WellTyped env x₂)
-  (h₃ : x₁.typeOf = .bool .anyBool)
-  (h₄ : x₂.typeOf = .bool .anyBool) :
-  WellTyped env (.or x₁ x₂ (.bool .anyBool))
-| unaryApp {op₁ : UnaryOp} {x₁ : TypedExpr}  {ty : CedarType}
-  (h₁ : WellTyped env x₁)
-  (h₂ : op₁.WellTyped x₁ ty) :
-  WellTyped env (.unaryApp op₁ x₁ ty)
-| binaryApp {op₂ : BinaryOp} {x₁ x₂: TypedExpr}  {ty : CedarType}
-  (h₁ : WellTyped env x₁)
-  (h₂ : WellTyped env x₂)
-  (h₃ : op₂.WellTyped env x₁ x₂ ty) :
-  WellTyped env (.binaryApp op₂ x₁ x₂ ty)
-| hasAttr_entity {ety : EntityType} {x₁ : TypedExpr} {attr : Attr}
-  (h₁ : WellTyped env x₁)
-  (h₂ : x₁.typeOf = .entity ety) :
-  WellTyped env (.hasAttr x₁ attr (.bool .anyBool))
-| hasAttr_record {rty : RecordType} {x₁ : TypedExpr} {attr : Attr}
-  (h₁ : WellTyped env x₁)
-  (h₂ : x₁.typeOf = .record rty) :
-  WellTyped env (.hasAttr x₁ attr (.bool .anyBool))
-| getAttr_entity {ety : EntityType} {rty : RecordType} {x₁ : TypedExpr} {attr : Attr} {ty : CedarType}
-  (h₁ : WellTyped env x₁)
-  (h₂ : x₁.typeOf = .entity ety)
-  (h₃ : env.ets.attrs? ety = .some rty)
-  (h₄ : (rty.find? attr).map Qualified.getType = .some ty) :
-  WellTyped env (.getAttr x₁ attr ty)
-| getAttr_record {rty : RecordType} {x₁ : TypedExpr} {attr : Attr} {ty : CedarType}
-  (h₁ : WellTyped env x₁)
-  (h₂ : x₁.typeOf = .record rty)
-  (h₃ : (rty.find? attr).map Qualified.getType = .some ty) :
-  WellTyped env (.getAttr x₁ attr ty)
-| set {ls : List TypedExpr} {ty : CedarType}
-  (h₁ : ∀ x, x ∈ ls → WellTyped env x)
-  (h₂ : ∀ x, x ∈ ls → x.typeOf = ty) :
-  WellTyped env (.set ls (.set ty))
-| record {rty : RecordType} {m : List (Attr × TypedExpr)}
-  (h₁ : ∀ k v, (k,v) ∈ m → WellTyped env v)
-  -- should we require well-formedness of `m` and then rewrite h₁ using quantifiers?
-  (h₂ : rty = Map.make (m.map (λ (a, ty) => (a, .required ty.typeOf)))) :
-  WellTyped env (.record m (.record rty))
-| call {xfn : ExtFun} {args : List TypedExpr} {ty : CedarType}
-  (h₁ : ∀ x, x ∈ args → WellTyped env x)
-  (h₂ : xfn.WellTyped args ty) :
-  WellTyped env (.call xfn args ty)
+theorem well_typed_is_sound {v : Value} {env : Environment} {ty : TypedExpr} {request : Request} {entities : Entities} :
+  RequestAndEntitiesMatchEnvironment env request entities →
+  TypedExpr.WellTyped env ty →
+  evaluate ty.toExpr request entities = .ok v →
+  InstanceOfType v ty.typeOf
+:= by
+  intro h₀ h₁ h₂
+  cases h₁ <;> try simp only [TypedExpr.toExpr, evaluate] at h₂
+  case lit p ty h₃ =>
+    cases h₃ <;>
+    simp only [TypedExpr.typeOf] <;>
+    simp only [Except.ok.injEq] at h₂ <;>
+    rw [←h₂]
+    case bool => simp only [bool_is_instance_of_anyBool]
+    case int => exact InstanceOfType.instance_of_int
+    case string => exact InstanceOfType.instance_of_string
+    case entityUID uid h =>
+      have : InstanceOfEntityType uid uid.ty := by rfl
+      exact InstanceOfType.instance_of_entity uid uid.ty this
+  case var h₃ =>
+    cases h₃ <;>
+    simp only [TypedExpr.typeOf] <;>
+    simp only [TypedExpr.toExpr, evaluate, Except.ok.injEq] at h₂ <;>
+    rw [←h₂] <;>
+    simp only [RequestAndEntitiesMatchEnvironment, InstanceOfRequestType] at h₀
+    case principal =>
+      rcases h₀ with ⟨⟨h₀, _, _, _⟩, _, _⟩
+      exact InstanceOfType.instance_of_entity request.principal env.reqty.principal h₀
+    case resource =>
+      rcases h₀ with ⟨⟨_, _, h₀, _⟩, _, _⟩
+      exact InstanceOfType.instance_of_entity request.resource env.reqty.resource h₀
+    case action =>
+      rcases h₀ with ⟨⟨_, h₀, _, _⟩, _, _⟩
+      simp only [h₀]
+      have : InstanceOfEntityType env.reqty.action env.reqty.action.ty := by rfl
+      exact InstanceOfType.instance_of_entity env.reqty.action env.reqty.action.ty this
+    case context =>
+      rcases h₀ with ⟨⟨_, _, _, h₀⟩, _, _⟩
+      exact h₀
+  case ite x₁ x₂ x₃ h₃ h₄ h₅ h₆ h₇ =>
+    generalize hᵢ₁ : evaluate x₁.toExpr request entities = res₁
+    cases res₁
+    case error => simp only [Result.as, hᵢ₁, Except.bind_err, reduceCtorEq] at h₂
+    case ok =>
+      rename_i v₁
+      have hᵢ₁' := well_typed_is_sound h₀ h₃ hᵢ₁
+      simp only [h₆] at hᵢ₁'
+      have ⟨b, hᵢ₁'⟩ := instance_of_anyBool_is_bool hᵢ₁'
+      simp only [hᵢ₁'] at hᵢ₁
+      simp only [Result.as, hᵢ₁, Coe.coe, Value.asBool, Except.bind_ok] at h₂
+      have : (TypedExpr.ite x₁ x₂ x₃ x₂.typeOf).typeOf = x₂.typeOf := by
+        simp only [TypedExpr.typeOf]
+      simp only [this]
+      cases b <;> simp at h₂
+      case false =>
+        have hᵢ₂ := well_typed_is_sound h₀ h₅ h₂
+        rw [←h₇] at hᵢ₂
+        exact hᵢ₂
+      case true =>
+        have hᵢ₃ := well_typed_is_sound h₀ h₄ h₂
+        exact hᵢ₃
+  case and x₁ x₂ h₃ h₄ h₅ h₆ =>
+    generalize hᵢ₁ : evaluate x₁.toExpr request entities = res₁
+    cases res₁
+    case error => simp only [Result.as, hᵢ₁, Except.bind_err, reduceCtorEq] at h₂
+    case ok =>
+      have hᵢ₁' := well_typed_is_sound h₀ h₃ hᵢ₁
+      simp only [h₅] at hᵢ₁'
+      have ⟨b, hᵢ₁'⟩ := instance_of_anyBool_is_bool hᵢ₁'
+      simp only [hᵢ₁'] at hᵢ₁
+      simp only [Result.as, hᵢ₁, Coe.coe, Value.asBool, Except.bind_ok] at h₂
+      simp only [TypedExpr.typeOf]
+      cases b <;> simp at h₂
+      case false =>
+        rw [←h₂]
+        simp only [bool_is_instance_of_anyBool]
+      case true =>
+        generalize hᵢ₂ : evaluate x₂.toExpr request entities = res₂
+        cases res₂
+        case error =>
+          simp only [hᵢ₂, Except.map_error, reduceCtorEq] at h₂
+        case ok =>
+          simp only [hᵢ₂] at h₂
+          have hᵢ₂' := well_typed_is_sound h₀ h₄ hᵢ₂
+          simp only [h₆] at hᵢ₂'
+          have ⟨_, hᵢ₂'⟩ := instance_of_anyBool_is_bool hᵢ₂'
+          simp only [hᵢ₂', Except.map_ok, Except.ok.injEq] at h₂
+          rw [←h₂]
+          simp only [bool_is_instance_of_anyBool]
+  case or x₁ x₂ h₃ h₄ h₅ h₆ =>
+    generalize hᵢ₁ : evaluate x₁.toExpr request entities = res₁
+    cases res₁
+    case error => simp only [Result.as, hᵢ₁, Except.bind_err, reduceCtorEq] at h₂
+    case ok =>
+      have hᵢ₁' := well_typed_is_sound h₀ h₃ hᵢ₁
+      simp only [h₅] at hᵢ₁'
+      have ⟨b, hᵢ₁'⟩ := instance_of_anyBool_is_bool hᵢ₁'
+      simp only [hᵢ₁'] at hᵢ₁
+      simp only [Result.as, hᵢ₁, Coe.coe, Value.asBool, Except.bind_ok] at h₂
+      simp only [TypedExpr.typeOf]
+      cases b <;> simp at h₂
+      case true =>
+        rw [←h₂]
+        simp only [bool_is_instance_of_anyBool]
+      case false =>
+        generalize hᵢ₂ : evaluate x₂.toExpr request entities = res₂
+        cases res₂
+        case error =>
+          simp only [hᵢ₂, Except.map_error, reduceCtorEq] at h₂
+        case ok =>
+          simp only [hᵢ₂] at h₂
+          have hᵢ₂' := well_typed_is_sound h₀ h₄ hᵢ₂
+          simp only [h₆] at hᵢ₂'
+          have ⟨_, hᵢ₂'⟩ := instance_of_anyBool_is_bool hᵢ₂'
+          simp only [hᵢ₂', Except.map_ok, Except.ok.injEq] at h₂
+          rw [←h₂]
+          simp only [bool_is_instance_of_anyBool]
+  case unaryApp op x₁ ty hᵢ h₃ =>
+    generalize hᵢ₁ : evaluate x₁.toExpr request entities = res₁
+    cases res₁
+    case error => simp only [Result.as, hᵢ₁, Except.bind_err, reduceCtorEq] at h₂
+    case ok v =>
+      simp only [hᵢ₁, apply₁, Except.bind_ok] at h₂
+      split at h₂ <;> cases h₃ <;> simp only [TypedExpr.typeOf]
+      · simp only [Except.ok.injEq] at h₂
+        rw [←h₂]
+        simp only [bool_is_instance_of_anyBool]
+      · simp only [intOrErr] at h₂
+        split at h₂
+        · simp only [Except.ok.injEq] at h₂
+          rw [←h₂]
+          exact InstanceOfType.instance_of_int
+        · cases h₂
+      · simp only [Except.ok.injEq] at h₂
+        rw [←h₂]
+        simp only [bool_is_instance_of_anyBool]
+      · simp only [Except.ok.injEq] at h₂
+        rw [←h₂]
+        simp only [bool_is_instance_of_anyBool]
+      · cases h₂
+      · cases h₂
+      · cases h₂
+      · cases h₂
+  case binaryApp op₂ x₁ x₂ ty hᵢ₁ hᵢ₂ h₃ =>
+    generalize hᵢ₁' : evaluate x₁.toExpr request entities = res₁
+    generalize hᵢ₂' : evaluate x₂.toExpr request entities = res₂
+    cases res₁ <;> cases res₂ <;> simp [hᵢ₁', hᵢ₂'] at h₂
+    -- case ok.ok
+    rename_i v₁ v₂
+    simp only [apply₂] at h₂
+    simp only [TypedExpr.typeOf]
+    split at h₂ <;>
+    cases h₃ <;>
+    try cases h₂ <;>
+    try simp only [bool_is_instance_of_anyBool]
+    · sorry
+    · sorry
+    · sorry
+    · sorry
+    · sorry
+    · sorry
+  case hasAttr_entity ety x₁ attr hᵢ h₃ =>
+    generalize hᵢ' : evaluate x₁.toExpr request entities = res₁
+    cases res₁ <;> simp [hᵢ'] at h₂
+    simp only [hasAttr] at h₂
+    sorry
+  case hasAttr_record => sorry
+  case getAttr_entity => sorry
+  case getAttr_record => sorry
+  case set => sorry
+  case record => sorry
+  case call xfn args ty h₃ h₄ => sorry
+    /-
+    generalize hᵢ : ((args.map₁ λ x => x.val.toExpr).mapM₁ λ x => evaluate x.val request entities) = res₁
+    cases res₁ <;> simp [hᵢ] at h₂
+    simp only [call, res, gt_iff_lt, ge_iff_le] at h₂
+    simp only [TypedExpr.typeOf]
+    split at h₂ <;>
+    cases h₄
+    case _ v _=>
+      sorry
+    case _ =>
+      simp only [Except.ok.injEq] at h₂
+      rw [←h₂]
+      simp only [bool_is_instance_of_anyBool]
+    case _ =>
+      simp only [Except.ok.injEq] at h₂
+      rw [←h₂]
+      simp only [bool_is_instance_of_anyBool]
+    case _ =>
+      simp only [Except.ok.injEq] at h₂
+      rw [←h₂]
+      simp only [bool_is_instance_of_anyBool]
+    case _ =>
+      simp only [Except.ok.injEq] at h₂
+      rw [←h₂]
+      simp only [bool_is_instance_of_anyBool]
+    case _ => sorry
+    case _ =>
+      simp only [Except.ok.injEq] at h₂
+      rw [←h₂]
+      simp only [bool_is_instance_of_anyBool]
+    case _ =>
+      simp only [Except.ok.injEq] at h₂
+      rw [←h₂]
+      simp only [bool_is_instance_of_anyBool]
+    case _ =>
+      simp only [Except.ok.injEq] at h₂
+      rw [←h₂]
+      simp only [bool_is_instance_of_anyBool]
+    case _ =>
+      simp only [Except.ok.injEq] at h₂
+      rw [←h₂]
+      simp only [bool_is_instance_of_anyBool]
+    case _ =>
+      simp only [Except.ok.injEq] at h₂
+      rw [←h₂]
+      simp only [bool_is_instance_of_anyBool]
+    case _ => sorry
+    case _ => sorry
+    case _ => sorry
+    case _ => sorry
+    case _ => sorry
+    case _ => sorry
+    case _ => sorry
+    case _ => cases h₂
+    case _ => cases h₂
+    case _ => cases h₂
+    case _ => cases h₂
+    case _ => cases h₂
+    case _ => cases h₂
+    case _ => cases h₂
+    case _ => cases h₂
+    case _ => cases h₂
+    case _ => cases h₂
+    case _ => cases h₂
+    case _ => cases h₂
+    case _ => cases h₂
+    case _ => cases h₂
+    case _ => cases h₂
+    case _ => cases h₂
+  -/
+
+theorem typechecked_is_well_typed_after_lifting {e : Expr} {c₁ c₂ : Capabilities} {env : Environment} {ty : TypedExpr} {request : Request} {entities : Entities} :
+  CapabilitiesInvariant c₁ request entities →
+  RequestAndEntitiesMatchEnvironment env request entities →
+  typeOf e c₁ env = .ok (ty, c₂) →
+  TypedExpr.WellTyped env ty.liftBoolTypes
+:= by sorry
 
 end Cedar.Thm
