cedar-lean/Cedar/Thm/Validation/WellTyped/Definition.lean
@@ -1,0 +1,269 @@
+/-
+ Copyright Cedar Contributors
+
+ Licensed under the Apache License, Version 2.0 (the "License");
+ you may not use this file except in compliance with the License.
+ You may obtain a copy of the License at
+
+      https://www.apache.org/licenses/LICENSE-2.0
+
+ Unless required by applicable law or agreed to in writing, software
+ distributed under the License is distributed on an "AS IS" BASIS,
+ WITHOUT WARRANTIES OR CONDITIONS OF ANY KIND, either express or implied.
+ See the License for the specific language governing permissions and
+ limitations under the License.
+-/
+import Cedar.Validation.TypedExpr
+import Cedar.Thm
+import Cedar.Spec.Ext
+
+/-!
+This file contains well-typedness definitions of `TypedExpr`
+-/
+
+namespace Cedar.Spec
+
+open Cedar.Validation
+open Cedar.Spec.Ext
+
+inductive Prim.WellTyped (env : Environment) : Prim → CedarType → Prop
+  | bool (b : Bool) :
+    WellTyped env (.bool b) (.bool .anyBool)
+  | int (i : Int64) :
+    WellTyped env (.int i) .int
+  | string (s : String) :
+    WellTyped env (.string s) .string
+  | entityUID (uid : EntityUID)
+    (h₁ : env.ets.isValidEntityUID uid || env.acts.contains uid) :
+    WellTyped env (.entityUID uid) (.entity uid.ty)
+
+inductive Var.WellTyped (env : Environment) : Var → CedarType → Prop
+  | principal :
+    WellTyped env .principal (.entity env.reqty.principal)
+  | resource :
+    WellTyped env .resource (.entity env.reqty.resource)
+  | action :
+    WellTyped env .action (.entity env.reqty.action.ty)
+  | context:
+    WellTyped env .context (.record env.reqty.context)
+
+inductive UnaryOp.WellTyped : UnaryOp → TypedExpr → CedarType → Prop
+  | not {x₁ : TypedExpr}
+    (h₁ : x₁.typeOf = .bool .anyBool) :
+    WellTyped .not x₁ (.bool .anyBool)
+  | neg {x₁ : TypedExpr}
+    (h₁ : x₁.typeOf = .int) :
+    WellTyped .neg x₁ .int
+  | isEmpty {x₁ : TypedExpr} {eltTy : CedarType}
+    (h₁ : x₁.typeOf = .set eltTy) :
+    WellTyped .isEmpty x₁ (.bool .anyBool)
+  | like {x₁ : TypedExpr} {p : Pattern}
+    (h₁ : x₁.typeOf = .string) :
+    WellTyped (.like p) x₁ (.bool .anyBool)
+
+inductive BinaryOp.WellTyped (env : Environment) : BinaryOp → TypedExpr → TypedExpr → CedarType → Prop
+  | eq {x₁ x₂ : TypedExpr}
+    (h₁ : x₁.typeOf = x₂.typeOf) :
+    WellTyped env .eq x₁ x₂ (.bool .anyBool)
+  | memₑ {x₁ x₂ : TypedExpr} {ety₁ ety₂ : EntityType}
+    (h₁ : x₁.typeOf = .entity ety₁)
+    (h₂ : x₂.typeOf = .entity ety₁) :
+    WellTyped env .mem x₁ x₂ (.bool .anyBool)
+  | memₛ {x₁ x₂ : TypedExpr} {ety₁ ety₂ : EntityType}
+    (h₁ : x₁.typeOf = .entity ety₁)
+    (h₂ : x₂.typeOf = .set (.entity ety₁)) :
+    WellTyped env .mem x₁ x₂ (.bool .anyBool)
+  | less_int {x₁ x₂ : TypedExpr}
+    (h₁ : x₁.typeOf = .int)
+    (h₂ : x₂.typeOf = .int) :
+    WellTyped env .less x₁ x₂ (.bool .anyBool)
+  | less_datetime {x₁ x₂ : TypedExpr}
+    (h₁ : x₁.typeOf = .ext .datetime)
+    (h₂ : x₂.typeOf = .ext .datetime) :
+    WellTyped env .less x₁ x₂ (.bool .anyBool)
+  | less_duration {x₁ x₂ : TypedExpr}
+    (h₁ : x₁.typeOf = .ext .duration)
+    (h₂ : x₂.typeOf = .ext .duration) :
+    WellTyped env .less x₁ x₂ (.bool .anyBool)
+  | lessEq_int {x₁ x₂ : TypedExpr}
+    (h₁ : x₁.typeOf = .int)
+    (h₂ : x₂.typeOf = .int) :
+    WellTyped env .lessEq x₁ x₂ (.bool .anyBool)
+  | lessEq_datetime {x₁ x₂ : TypedExpr}
+    (h₁ : x₁.typeOf = .ext .datetime)
+    (h₂ : x₂.typeOf = .ext .datetime) :
+    WellTyped env .lessEq x₁ x₂ (.bool .anyBool)
+  | lessEq_duration {x₁ x₂ : TypedExpr}
+    (h₁ : x₁.typeOf = .ext .duration)
+    (h₂ : x₂.typeOf = .ext .duration) :
+    WellTyped env .lessEq x₁ x₂ (.bool .anyBool)
+  | add {x₁ x₂ : TypedExpr}
+    (h₁ : x₁.typeOf = .int)
+    (h₂ : x₂.typeOf = .int) :
+    WellTyped env .add x₁ x₂ .int
+  | sub {x₁ x₂ : TypedExpr}
+    (h₁ : x₁.typeOf = .int)
+    (h₂ : x₂.typeOf = .int) :
+    WellTyped env .sub x₁ x₂ .int
+  | mul {x₁ x₂ : TypedExpr}
+    (h₁ : x₁.typeOf = .int)
+    (h₂ : x₂.typeOf = .int) :
+    WellTyped env .mul x₁ x₂ .int
+  | contains {x₁ x₂ : TypedExpr}
+    (h₁ : x₁.typeOf = .set x₂.typeOf) :
+    WellTyped env .contains x₁ x₂ (.bool .anyBool)
+  | containsAll {x₁ x₂ : TypedExpr} {ty : CedarType}
+    (h₁ : x₁.typeOf = .set ty)
+    (h₂ : x₂.typeOf = .set ty) :
+    WellTyped env .containsAll x₁ x₂ (.bool .anyBool)
+  | containsAny {x₁ x₂ : TypedExpr} {ty : CedarType}
+    (h₁ : x₁.typeOf = .set ty)
+    (h₂ : x₂.typeOf = .set ty) :
+    WellTyped env .containsAny x₁ x₂ (.bool .anyBool)
+  | hasTag {x₁ x₂ : TypedExpr} {ety : EntityType}
+    (h₁ : x₁.typeOf = .entity ety)
+    (h₂ : x₂.typeOf = .string) :
+    WellTyped env .hasTag x₁ x₂ (.bool .anyBool)
+  | getTag {x₁ x₂ : TypedExpr} {ety : EntityType}
+    (h₁ : x₁.typeOf = .entity ety)
+    (h₂ : x₂.typeOf = .string)
+    (h₃ : env.ets.tags? ety = .some (.some ty)) :
+    WellTyped env .getTag x₁ x₂ ty
+
+inductive ExtFun.WellTyped : ExtFun → List TypedExpr → CedarType → Prop
+  | decimal {s₁ : String} {d₁ : Decimal}
+    (h₁ : d₁ = Decimal.decimal s₁) :
+    WellTyped .decimal [.lit (.string s₁) .string] (.ext .decimal)
+  | lessThan {x₁ x₂ : TypedExpr}
+    (h₁ : x₁.typeOf = .ext .decimal)
+    (h₂ : x₂.typeOf = .ext .decimal) :
+    WellTyped .lessThan [x₁, x₂] (.bool .anyBool)
+  | lessThanOrEqual {x₁ x₂ : TypedExpr}
+    (h₁ : x₁.typeOf = .ext .decimal)
+    (h₂ : x₂.typeOf = .ext .decimal) :
+    WellTyped .lessThan [x₁, x₂] (.bool .anyBool)
+  | greaterThan {x₁ x₂ : TypedExpr}
+    (h₁ : x₁.typeOf = .ext .decimal)
+    (h₂ : x₂.typeOf = .ext .decimal) :
+    WellTyped .lessThan [x₁, x₂] (.bool .anyBool)
+  | greaterThanOrEqual {x₁ x₂ : TypedExpr}
+    (h₁ : x₁.typeOf = .ext .decimal)
+    (h₂ : x₂.typeOf = .ext .decimal) :
+    WellTyped .lessThan [x₁, x₂] (.bool .anyBool)
+  | ip {s₁ : String} {ip₁ : IPAddr}
+    (h₁ : ip₁ =  IPAddr.ip s₁) :
+    WellTyped .ip [.lit (.string s₁) .string] (.ext .ipAddr)
+  | isIpv4 {x₁ : TypedExpr}
+    (h₁ : x₁.typeOf = .ext .ipAddr) :
+    WellTyped .isIpv4 [x₁] (.bool .anyBool)
+  | isIpv6 {x₁ : TypedExpr}
+    (h₁ : x₁.typeOf = .ext .ipAddr) :
+    WellTyped .isIpv6 [x₁] (.bool .anyBool)
+  | isLoopback {x₁ : TypedExpr}
+    (h₁ : x₁.typeOf = .ext .ipAddr) :
+    WellTyped .isLoopback [x₁] (.bool .anyBool)
+  | isMulticast {x₁ : TypedExpr}
+    (h₁ : x₁.typeOf = .ext .ipAddr) :
+    WellTyped .isMulticast [x₁] (.bool .anyBool)
+  | isInRange {x₁ x₂ : TypedExpr}
+    (h₁ : x₁.typeOf = .ext .ipAddr)
+    (h₂ : x₂.typeOf = .ext .ipAddr):
+    WellTyped .isInRange [x₁, x₂] (.bool .anyBool)
+  | datetime {s₁ : String} {d₁ : Datetime}
+    (h₁ : d₁ =  Datetime.parse s₁) :
+    WellTyped .datetime [.lit (.string s₁) .string] (.ext .datetime)
+  | duration {s₁ : String} {d₁ : Duration}
+    (h₁ : d₁ =  Datetime.Duration.parse s₁) :
+    WellTyped .duration [.lit (.string s₁) .string] (.ext .duration)
+  | offset {x₁ x₂ : TypedExpr}
+    (h₁ : x₁.typeOf = .ext .datetime)
+    (h₂ : x₂.typeOf = .ext .duration):
+    WellTyped .offset [x₁, x₂] (.ext .datetime)
+  | durationSince {x₁ x₂ : TypedExpr}
+    (h₁ : x₁.typeOf = .ext .datetime)
+    (h₂ : x₂.typeOf = .ext .datetime):
+    WellTyped .durationSince [x₁, x₂] (.ext .duration)
+  | toDate {x₁ : TypedExpr}
+    (h₁ : x₁.typeOf = .ext .datetime) :
+    WellTyped .toDate [x₁] (.ext .datetime)
+  | toTime {x₁ : TypedExpr}
+    (h₁ : x₁.typeOf = .ext .datetime) :
+    WellTyped .toTime [x₁] (.ext .duration)
+
+end Cedar.Spec
+
+namespace Cedar.Thm
+
+open Cedar.Validation
+open Cedar.Spec
+open Cedar.Data
+
+inductive TypedExpr.WellTyped (env : Environment) : TypedExpr → Prop
+| lit {p : Prim} {ty : CedarType}
+  (h₁ : p.WellTyped env ty) :
+  WellTyped env (.lit p ty)
+| var {v : Var} {ty : CedarType}
+  (h₁ : v.WellTyped env ty) :
+  WellTyped env (.var v ty)
+| ite {x₁ x₂ x₃ : TypedExpr}
+  (h₁ : WellTyped env x₁)
+  (h₂ : WellTyped env x₂)
+  (h₃ : WellTyped env x₃)
+  (h₄ : x₁.typeOf = .bool .anyBool)
+  (h₅ : x₂.typeOf = x₃.typeOf) :
+  WellTyped env (.ite x₁ x₂ x₃ x₂.typeOf)
+| and {x₁ x₂ : TypedExpr}
+  (h₁ : WellTyped env x₁)
+  (h₂ : WellTyped env x₂)
+  (h₃ : x₁.typeOf = .bool .anyBool)
+  (h₄ : x₂.typeOf = .bool .anyBool) :
+  WellTyped env (.and x₁ x₂ (.bool .anyBool))
+| or {x₁ x₂ : TypedExpr}
+  (h₁ : WellTyped env x₁)
+  (h₂ : WellTyped env x₂)
+  (h₃ : x₁.typeOf = .bool .anyBool)
+  (h₄ : x₂.typeOf = .bool .anyBool) :
+  WellTyped env (.or x₁ x₂ (.bool .anyBool))
+| unaryApp {op₁ : UnaryOp} {x₁ : TypedExpr}  {ty : CedarType}
+  (h₁ : WellTyped env x₁)
+  (h₂ : op₁.WellTyped x₁ ty) :
+  WellTyped env (.unaryApp op₁ x₁ ty)
+| binaryApp {op₂ : BinaryOp} {x₁ x₂: TypedExpr}  {ty : CedarType}
+  (h₁ : WellTyped env x₁)
+  (h₂ : WellTyped env x₂)
+  (h₃ : op₂.WellTyped env x₁ x₂ ty) :
+  WellTyped env (.binaryApp op₂ x₁ x₂ ty)
+| hasAttr_entity {ety : EntityType} {x₁ : TypedExpr} {attr : Attr}
+  (h₁ : WellTyped env x₁)
+  (h₂ : x₁.typeOf = .entity ety) :
+  WellTyped env (.hasAttr x₁ attr (.bool .anyBool))
+| hasAttr_record {rty : RecordType} {x₁ : TypedExpr} {attr : Attr}
+  (h₁ : WellTyped env x₁)
+  (h₂ : x₁.typeOf = .record rty) :
+  WellTyped env (.hasAttr x₁ attr (.bool .anyBool))
+| getAttr_entity {ety : EntityType} {rty : RecordType} {x₁ : TypedExpr} {attr : Attr} {ty : CedarType}
+  (h₁ : WellTyped env x₁)
+  (h₂ : x₁.typeOf = .entity ety)
+  (h₃ : env.ets.attrs? ety = .some rty)
+  (h₄ : (rty.find? attr).map Qualified.getType = .some ty) :
+  WellTyped env (.getAttr x₁ attr ty)
+| getAttr_record {rty : RecordType} {x₁ : TypedExpr} {attr : Attr} {ty : CedarType}
+  (h₁ : WellTyped env x₁)
+  (h₂ : x₁.typeOf = .record rty)
+  (h₃ : (rty.find? attr).map Qualified.getType = .some ty) :
+  WellTyped env (.getAttr x₁ attr ty)
+| set {ls : List TypedExpr} {ty : CedarType}
+  (h₁ : ∀ x, x ∈ ls → WellTyped env x)
+  (h₂ : ∀ x, x ∈ ls → x.typeOf = ty) :
+  WellTyped env (.set ls (.set ty))
+| record {rty : RecordType} {m : List (Attr × TypedExpr)}
+  (h₁ : ∀ k v, (k,v) ∈ m → WellTyped env v)
+  -- should we require well-formedness of `m` and then rewrite h₁ using quantifiers?
+  (h₂ : rty = Map.make (m.map (λ (a, ty) => (a, .required ty.typeOf)))) :
+  WellTyped env (.record m (.record rty))
+| call {xfn : ExtFun} {args : List TypedExpr} {ty : CedarType}
+  (h₁ : ∀ x, x ∈ args → WellTyped env x)
+  (h₂ : xfn.WellTyped args ty) :
+  WellTyped env (.call xfn args ty)
+
+end Cedar.Thm
