cedar-lean/Cedar/Thm/Validation/WellTyped/TypeLifting.lean
@@ -1,0 +1,86 @@
+/-
+ Copyright Cedar Contributors
+
+ Licensed under the Apache License, Version 2.0 (the "License");
+ you may not use this file except in compliance with the License.
+ You may obtain a copy of the License at
+
+      https://www.apache.org/licenses/LICENSE-2.0
+
+ Unless required by applicable law or agreed to in writing, software
+ distributed under the License is distributed on an "AS IS" BASIS,
+ WITHOUT WARRANTIES OR CONDITIONS OF ANY KIND, either express or implied.
+ See the License for the specific language governing permissions and
+ limitations under the License.
+-/
+
+import Cedar.Validation.TypedExpr
+import Cedar.Spec
+
+/-!
+This file contains theorems related to `TypedExpr.liftBoolTypes`
+-/
+
+namespace Cedar.Thm
+
+open Cedar.Validation
+open Cedar.Spec
+
+theorem type_lifting_preserves_expr (x : TypedExpr):
+  x.toExpr = x.liftBoolTypes.toExpr
+:= by
+  cases x <;> simp only [TypedExpr.toExpr, TypedExpr.liftBoolTypes]
+  case ite a b c _ =>
+    simp only [type_lifting_preserves_expr a, type_lifting_preserves_expr b, type_lifting_preserves_expr c]
+  case and a b _ =>
+    simp only [type_lifting_preserves_expr a, type_lifting_preserves_expr b]
+  case or a b _ =>
+    simp only [type_lifting_preserves_expr a, type_lifting_preserves_expr b]
+  case unaryApp a _ =>
+    simp only [type_lifting_preserves_expr a]
+  case binaryApp a b _ =>
+    simp only [type_lifting_preserves_expr a, type_lifting_preserves_expr b]
+  case getAttr a _ _ =>
+    simp only [type_lifting_preserves_expr a]
+  case hasAttr a _ _ =>
+    simp only [type_lifting_preserves_expr a]
+  case set s _ =>
+    simp only [List.map₁_eq_map, List.map_map, Expr.set.injEq, List.map_inj_left,
+      Function.comp_apply]
+    exact λ x _ => type_lifting_preserves_expr x
+  case record m _ =>
+    simp only [Expr.record.injEq]
+    have : m.attach₂.map (λ x => (x.1.fst, x.1.snd.toExpr)) =
+      m.map λ x => (x.fst, x.snd.toExpr) := by
+      exact List.map_attach₂ λ x : Attr × TypedExpr => (x.fst, x.snd.toExpr)
+    rw [this]
+    have : m.attach₂.map (λ x => (x.1.fst, x.1.snd.liftBoolTypes)) =
+      m.map λ x => (x.fst, x.snd.liftBoolTypes) := by
+      exact List.map_attach₂ λ x : Attr × TypedExpr => (x.fst, x.snd.liftBoolTypes)
+    rw [this]
+    have : (List.map (λ x => (x.fst, x.snd.liftBoolTypes)) m).attach₂.map (λ x => (x.1.fst, x.1.snd.toExpr)) =
+      (List.map (λ x => (x.fst, x.snd.liftBoolTypes)) m).map (λ x => (x.fst, x.snd.toExpr)) := by
+      exact List.map_attach₂ λ x : Attr × TypedExpr => (x.fst, x.snd.toExpr)
+    rw [this]
+    simp only [List.map_map, List.map_inj_left, Function.comp_apply, Prod.mk.injEq, true_and,
+      Prod.forall]
+    exact λ _ x _ => type_lifting_preserves_expr x
+  case call args _ =>
+    simp only [List.map₁_eq_map, List.map_map, Expr.call.injEq, List.map_inj_left,
+      Function.comp_apply, true_and]
+    exact λ x _ => type_lifting_preserves_expr x
+  termination_by x
+  decreasing_by
+    all_goals (simp_wf ; try omega)
+    all_goals
+      rename_i h
+      have := List.sizeOf_lt_of_mem h
+      simp only [Prod.mk.sizeOf_spec] at this
+      omega
+
+theorem type_lifting_preserves_evaluation_results {x : TypedExpr} {request : Request} {entities : Entities} :
+  evaluate x.toExpr request entities = evaluate x.liftBoolTypes.toExpr request entities
+ := by
+ simp only [type_lifting_preserves_expr x]
+
+end Cedar.Thm
